<h1 align="Center">𝑨𝒓𝒊𝒕𝒉𝒎𝒆𝒕𝒊𝒄 𝑬𝒙𝒑𝒓𝒆𝒔𝒔𝒊𝒐𝒏</h1>

<ul>
  
<h3> 𝑳𝒆𝒕 𝑸 𝒃𝒆 𝒂𝒏 𝒂𝒓𝒊𝒕𝒉𝒎𝒆𝒕𝒊𝒄 𝒆𝒙𝒑𝒓𝒆𝒔𝒔𝒊𝒐𝒏 𝒊𝒏𝒗𝒐𝒍𝒗𝒊𝒏𝒈 𝒄𝒐𝒏𝒔𝒕𝒂𝒏𝒕𝒔
𝒂𝒏𝒅 𝒐𝒑𝒆𝒓𝒂𝒕𝒊𝒐𝒏𝒔 .</h3>
  
 ![Screenshot (508)](https://github.com/AvinandanBose/ArithmeticExp_Infix_Prefix_Postfix_Theory/assets/38869235/7cca382b-8e1b-4d1b-a2c8-b40f7c26cb6a)

<h3><ins>𝑵𝒐𝒕𝒆</ins> ∶ 𝑨𝒄𝒄𝒐𝒓𝒅𝒊𝒏𝒈 𝒕𝒐 𝒓𝒖𝒍𝒆𝒔 ∶ 𝑺𝒖𝒄𝒉 𝒂𝒔 𝑩𝑬𝑫𝑴𝑨𝑺(
𝑩𝒓𝒂𝒄𝒌𝒆𝒕𝒔, 𝑬𝒙𝒑𝒐𝒏𝒆𝒏𝒕𝒔, 𝑫𝒊𝒗𝒊𝒔𝒊𝒐𝒏, 𝑴𝒖𝒍𝒕𝒊𝒑𝒍𝒊𝒄𝒂𝒕𝒊𝒐𝒏,𝑨𝒅𝒅𝒊𝒕𝒊𝒐𝒏,
𝑺𝒖𝒃𝒕𝒓𝒂𝒄𝒕𝒊𝒐𝒏 ) 𝒇𝒐𝒍𝒍𝒐𝒘𝒆𝒅 𝒊𝒏 𝑪𝒂𝒏𝒂𝒅𝒂 .
𝑨𝒏𝒅 𝒊𝒏 𝑼𝑲,𝑷𝒂𝒌𝒊𝒔𝒕𝒂𝒏, 𝑰𝒏𝒅𝒊𝒂, 𝑩𝒂𝒏𝒈𝒍𝒂𝒅𝒆𝒔𝒉 𝒂𝒏𝒅
𝑨𝒖𝒔𝒕𝒓𝒂𝒍𝒊𝒂 𝒊𝒕𝒔 𝒇𝒐𝒍𝒍𝒐𝒘𝒆𝒅 𝑩𝑶𝑫𝑴𝑨𝑺 𝒎𝒆𝒂𝒏𝒊𝒏𝒈
𝑩𝒓𝒂𝒄𝒌𝒆𝒕𝒔, 𝑶𝒇, 𝑫𝒊𝒗𝒊𝒔𝒊𝒐𝒏, 𝑴𝒖𝒍𝒕𝒊𝒑𝒍𝒊𝒄𝒂𝒕𝒊𝒐𝒏,𝑨𝒅𝒅𝒊𝒕𝒊𝒐𝒏 𝒂𝒏𝒅
𝑺𝒖𝒃𝒕𝒓𝒂𝒄𝒕𝒊𝒐𝒏.</h3>

 <h3>𝑻𝒉𝒆 𝒆𝒙𝒑𝒓𝒆𝒔𝒔𝒊𝒐𝒏 𝒊𝒏 𝑩𝒓𝒂𝒄𝒌𝒆𝒕𝒔 𝒎𝒖𝒔𝒕 𝒃𝒆 𝒆𝒙𝒆𝒄𝒖𝒕𝒆𝒅 𝒂𝒕 𝒇𝒊𝒓𝒔𝒕.</h3>
  
 </ul>
 
   <h1></h1>
 <h1 align="Center">𝑰𝒏𝒇𝒊𝒙 𝑵𝒐𝒕𝒂𝒕𝒊𝒐𝒏</h1>
 
 <ul>
  
 <h3>𝑰𝒏 𝒕𝒉𝒊𝒔 𝒏𝒐𝒕𝒂𝒕𝒊𝒐𝒏 , 𝒕𝒉𝒆 𝒐𝒑𝒆𝒓𝒂𝒕𝒐𝒓 𝒊𝒔
𝒑𝒍𝒂𝒄𝒆𝒅 𝒃𝒆𝒕𝒘𝒆𝒆𝒏 𝒊𝒕𝒔 𝒕𝒘𝒐 𝒐𝒑𝒆𝒓𝒂𝒏𝒅𝒔. </h3>
  
  
 <h3>𝑬𝒈:</h3>
  
  <ul>
    
<h3><li>𝟏)𝑻𝒐 𝒂𝒅𝒅 𝑨 𝒕𝒐 𝑩 𝒘𝒆 𝒄𝒂𝒏 𝒘𝒓𝒊𝒕𝒆 𝒂𝒔: 𝑨 + 𝑩</li></h3>
<h3><li>𝟐) 𝑻𝒐 𝒔𝒖𝒃𝒕𝒓𝒂𝒄𝒕 𝑫 𝒇𝒓𝒐𝒎 𝑪 𝒘𝒆 𝒘𝒓𝒊𝒕𝒆 𝒂𝒔:
𝑪 − 𝑫.</li></h3>
    
<h3><li>𝑺𝒊𝒎𝒊𝒍𝒂𝒓𝒍𝒚, (𝑨 + 𝑩)/𝑪 𝒂𝒏𝒅 𝑨 + (𝑩/𝑪)</li></h3>

  </ul>
  
  <h1></h1>
  <h1 align="Center"> 𝑷𝒓𝒆𝒇𝒊𝒙 𝑵𝒐𝒕𝒂𝒕𝒊𝒐𝒏</h1>
  
  <ul>
    
  <h3>𝑰𝒏 𝒕𝒉𝒊𝒔 𝒏𝒐𝒕𝒂𝒕𝒊𝒐𝒏, 𝒏𝒂𝒎𝒆𝒅 𝒂𝒇𝒕𝒆𝒓 𝒕𝒉𝒆 𝑷𝒐𝒍𝒊𝒔𝒉 𝒎𝒂𝒕𝒉𝒆𝒎𝒂𝒕𝒊𝒄𝒊𝒂𝒏
𝑱𝒂𝒏 𝑳𝒖𝒌𝒂𝒔𝒊𝒆𝒘𝒊𝒄𝒛, 𝒕𝒉𝒆 𝒐𝒑𝒆𝒓𝒂𝒕𝒐𝒓 𝒔𝒚𝒎𝒃𝒐𝒍 𝒊𝒔 𝒑𝒍𝒂𝒄𝒆𝒅 𝒃𝒆𝒇𝒐𝒓𝒆 𝒊𝒕𝒔
𝒕𝒘𝒐 𝒐𝒑𝒆𝒓𝒂𝒏𝒅𝒔 .</h3>
    
 <h3><ins> 𝑭𝒐𝒓 𝒆𝒙𝒂𝒎𝒑𝒍𝒆 ,</ins></h3>
    
 <ul>
    
 <h3>→ 𝑻𝒐 𝒂𝒅𝒅 𝑨 𝒕𝒐 𝑩 𝒘𝒆 𝒄𝒂𝒏 𝒘𝒓𝒊𝒕𝒆 𝒂𝒔: + 𝑨𝑩 𝒐𝒓 + 𝑩𝑨.</h3>
<h3>→ 𝑻𝒐 𝒔𝒖𝒃𝒔𝒕𝒓𝒂𝒄𝒕 𝑫 𝒇𝒓𝒐𝒎 𝑪 𝒘𝒆 𝒉𝒂𝒗𝒆 𝒕𝒐 𝒘𝒓𝒊𝒕𝒆 𝒂𝒔 − 𝑪𝑫 .
𝑰𝒏 𝒐𝒓𝒅𝒆𝒓 𝒕𝒐 𝒕𝒓𝒂𝒏𝒔𝒍𝒂𝒕𝒆 𝒂𝒏 𝒂𝒓𝒊𝒕𝒉𝒎𝒆𝒕𝒊𝒄 𝒆𝒙𝒑𝒓𝒆𝒔𝒔𝒊𝒐𝒏 𝒊𝒏 𝒊𝒏𝒇𝒊𝒙
𝒏𝒐𝒕𝒂𝒕𝒊𝒐𝒏 𝒕𝒐 𝒑𝒐𝒍𝒊𝒔𝒉 𝒏𝒐𝒕𝒂𝒕𝒊𝒐𝒏, 𝒘𝒆 𝒅𝒐 𝒔𝒕𝒆𝒑 𝒃𝒚 𝒔𝒕𝒆𝒑 𝒖𝒔𝒊𝒏𝒈
𝒃𝒓𝒂𝒄𝒌𝒆𝒕𝒔([] ) 𝒕𝒐 𝒊𝒏𝒅𝒊𝒄𝒂𝒕𝒆 𝒕𝒉𝒆 𝒑𝒂𝒓𝒕𝒊𝒂𝒍 𝒕𝒓𝒂𝒏𝒔𝒍𝒂𝒕𝒊𝒐𝒏.</h3>
   
   
<h3>𝑪𝒐𝒏𝒔𝒊𝒅𝒆𝒓 𝒕𝒉𝒆 𝒇𝒐𝒍𝒍𝒐𝒘𝒊𝒏𝒈 𝒆𝒙𝒑𝒓𝒆𝒔𝒔𝒊𝒐𝒏 𝒊𝒏 𝒊𝒏𝒇𝒊𝒙 𝒏𝒐𝒕𝒂𝒕𝒊𝒐𝒏:</h3>
   
 <h3>
	
 ```math
	
 \begin{equation}
   \begin{split}
	
(𝑨 − 𝑩/𝑪) ∗ (𝑨 ∗ 𝑲 − 𝑳)\\	
	
    \end{split}
 \end{equation}
	
```

</h3>
   
<h3>𝒑𝒂𝒓𝒕𝒊𝒂𝒍 𝒕𝒓𝒂𝒏𝒔𝒍𝒂𝒕𝒊𝒐𝒏𝒔 𝒎𝒂𝒚 𝒍𝒐𝒐𝒌 𝒍𝒊𝒌𝒆:</h3>
   
 <h3>
	
 ```math
	
 \begin{equation}
   \begin{split}
	
= (𝑨 − [/𝑩𝑪]) ∗ ([∗ 𝑨𝑲] − 𝑳)\\
= [−𝑨/𝑩𝑪] ∗ [− ∗ 𝑨𝑲𝑳]\\
= ∗ −𝑨/𝑩𝑪 −∗ 𝑨𝑲𝑳	\\
	
    \end{split}
 \end{equation}
	
```

</h3>
   
<h2><ins>𝑬𝒙𝒂𝒎𝒑𝒍𝒆 𝟏:</ins></h2>
 
   
 <h3>
	
 ```math
	
 \begin{equation}
   \begin{split}
	
 𝑨 + ( 𝑩 ∗ 𝑪 – ( 𝑫/𝑬 + 𝑭) ∗ 𝑮) ∗𝑯\\	
	
    \end{split}
 \end{equation}
	
```

</h3>
  

   
<h3>𝑷𝒂𝒓𝒕𝒊𝒂𝒍 𝒕𝒓𝒂𝒏𝒔𝒍𝒂𝒕𝒊𝒐𝒏𝒔 𝒐𝒇 𝒕𝒉𝒆 𝒂𝒃𝒐𝒗𝒆:</h3>
  
<ul>
   
<h3>𝟏𝒔𝒕 𝒘𝒆 𝒘𝒊𝒍𝒍 𝒅𝒐 𝒕𝒉𝒆 𝒘𝒐𝒓𝒌 𝒐𝒇 𝑷𝒂𝒓𝒆𝒏𝒕𝒉𝒆𝒔𝒊𝒔.</h3>
<h3>𝑵𝒆𝒙𝒕 𝒘𝒆 𝒘𝒊𝒍𝒍 𝒇𝒐𝒍𝒍𝒐𝒘 𝒕𝒉𝒆 𝒑𝒓𝒆𝒄𝒆𝒅𝒆𝒏𝒄𝒆 𝒕𝒂𝒃𝒍𝒆:</h3>

 ![Screenshot (509)](https://github.com/AvinandanBose/ArithmeticExp_Infix_Prefix_Postfix_Theory/assets/38869235/48e06f23-b88f-4ef2-a539-98d4de1d10d9)
  
<h3>𝑯𝒊𝒈𝒉𝒆𝒔𝒕 𝒑𝒓𝒆𝒄𝒆𝒅𝒆𝒏𝒄𝒆 𝒘𝒊𝒍𝒍 𝒃𝒆 𝒆𝒙𝒆𝒄𝒖𝒕𝒆𝒅 𝒇𝒊𝒓𝒔𝒕 𝒂𝒏𝒅 𝒍𝒐𝒘𝒆𝒔𝒕 𝒂𝒕 𝒍𝒂𝒔𝒕.</h3>


</ul>
   
<h3>
	
 ```math
	
 \begin{equation}
   \begin{split}
	
= 𝑨 + ( 𝑩 ∗ 𝑪 – ( [/𝑫𝑬] + 𝑭) ∗ 𝑮) ∗ 𝑯 \quad \quad \quad \quad \quad \quad \quad \quad \quad \\
[/𝑫𝑬 \quad 𝒊𝒔 \quad 𝒑𝒓𝒆𝒇𝒊𝒙 \quad 𝒔𝒕𝒓𝒊𝒏𝒈 \quad + 𝑭 \quad 𝒊𝒔 \quad 𝒔𝒕𝒊𝒍𝒍 \quad 𝒂𝒏 \quad 𝒊𝒏𝒇𝒊𝒙 \quad 𝒔𝒕𝒓𝒊𝒏𝒈.]\\
= 𝑨 + ( 𝑩 ∗ 𝑪 – ( [+/𝑫𝑬𝑭]) ∗ 𝑮) ∗ 𝑯 \quad \quad \quad \quad \quad \quad \quad \quad \quad  \\
= 𝑨 + ( 𝑩 ∗ 𝑪 – +/𝑫𝑬𝑭 ∗ 𝑮) ∗ 𝑯 \quad \quad \quad \quad \quad \quad \quad \quad \quad \\
[+/𝑫𝑬𝑭 \quad 𝒊𝒔 \quad 𝒑𝒓𝒆𝒇𝒊𝒙 \quad 𝒔𝒕𝒓𝒊𝒏𝒈 \quad ∗ 𝑮 \quad 𝒊𝒔 \quad 𝒔𝒕𝒊𝒍𝒍 \quad 𝒂𝒏 \quad 𝒊𝒏𝒇𝒊𝒙 \quad 𝒔𝒕𝒓𝒊𝒏𝒈.] \\
= 𝑨 + ( 𝑩 ∗ 𝑪 – [∗ +/𝑫𝑬𝑭𝑮]) ∗ 𝑯 \quad \quad \quad \quad \quad \quad \quad \quad \quad  \\
= 𝑨 + ([∗ 𝑩 𝑪] – [∗ +/𝑫𝑬𝑭𝑮]) ∗ 𝑯 \quad \quad \quad \quad \quad \quad \quad \quad \quad \\
= 𝑨 + ([− ∗ 𝑩 𝑪 ∗ +/𝑫𝑬𝑭𝑮]) ∗ 𝑯 \quad \quad \quad \quad \quad \quad \quad \quad \quad \\
= 𝑨 + − ∗ 𝑩 𝑪 ∗ +/𝑫𝑬𝑭𝑮 ∗ 𝑯 \quad \quad \quad \quad \quad \quad \quad \quad \quad \\
= 𝑨 + [∗ − ∗ 𝑩 𝑪 ∗ +/𝑫𝑬𝑭𝑮𝑯] \quad \quad \quad \quad \quad \quad \quad \quad \quad \\
= [+𝑨 ∗ − ∗ 𝑩 𝑪 ∗ +/𝑫𝑬𝑭𝑮𝑯] \quad \quad \quad \quad \quad \quad \quad \quad \quad \\
= +𝑨 ∗ − ∗ 𝑩 𝑪 ∗ +/𝑫𝑬𝑭𝑮𝑯 \quad \quad \quad \quad \quad \quad \quad \quad \quad \\
	
    \end{split}
 \end{equation}
	
```

</h3>
   
</ul>
    
    
<h2><ins>𝑬𝒙𝒂𝒎𝒑𝒍𝒆  𝟐:</ins></h2>
 
<h3>
  
<ul>
  
 ```Syntax
	
𝑨^𝑩 + 𝑪 ∗ 𝑫%𝑬 − 𝑭/𝑮
  
𝑷𝒂𝒓𝒕𝒊𝒂𝒍 𝒕𝒓𝒂𝒏𝒔𝒍𝒂𝒕𝒊𝒐𝒏𝒔 𝒐𝒇 𝒕𝒉𝒆 𝒂𝒃𝒐𝒗𝒆:
= [^𝑨𝑩] + 𝑪 ∗ 𝑫%𝑬 − 𝑭/𝑮
= ^𝑨𝑩 + 𝑪 ∗ 𝑫%𝑬 − [/𝑭𝑮]
= ^𝑨𝑩 + [∗ 𝑪𝑫]%𝑬 −/𝑭𝑮
= ^𝑨𝑩 +∗ 𝑪[%𝑫𝑬] −/𝑭𝑮
= ^𝑨𝑩 +∗ 𝑪%𝑫𝑬 −/𝑭𝑮
= [+^𝑨𝑩 ∗ 𝑪]%𝑫𝑬 −/𝑭𝑮
= +^𝑨𝑩 ∗ 𝑪%𝑫𝑬 −/𝑭𝑮[𝟏𝒔𝒕 𝒑𝒂𝒓𝒕:∗ 𝑪%𝑫𝑬 𝒂𝒏𝒅 𝟐𝒏𝒅 𝒑𝒂𝒓𝒕:/𝑭𝑮
𝒂𝒏𝒅 𝒐𝒑𝒆𝒓𝒂𝒕𝒐𝒓 = −]
= +^𝑨𝑩[− ∗ 𝑪%𝑫𝑬/𝑭𝑮]
= +^𝑨𝑩 −∗ 𝑪%𝑫𝑬/𝑭𝑮
	
```

</h3>
  
</ul>
    
</ul>
  
  <h1></h1>
  <h1 align="Center"> 𝑹𝒆𝒗𝒆𝒓𝒔𝒆 𝑷𝒐𝒍𝒊𝒔𝒉 (𝑷𝒐𝒔𝒕𝒇𝒊𝒙)𝑵𝒐𝒕𝒂𝒕𝒊𝒐𝒏</h1>
  
  <ul>
    
<h3>𝑰𝒏 𝒕𝒉𝒊𝒔 𝒏𝒐𝒕𝒂𝒕𝒊𝒐𝒏 𝒕𝒉𝒆 𝒐𝒑𝒆𝒓𝒂𝒕𝒐𝒓 𝒔𝒚𝒎𝒃𝒐𝒍 𝒊𝒔 𝒑𝒍𝒂𝒄𝒆𝒅 𝒂𝒇𝒕𝒆𝒓 𝒊𝒕𝒔
𝒕𝒘𝒐 𝒐𝒑𝒆𝒓𝒂𝒏𝒅𝒔. 𝑭𝒐𝒓 𝒆𝒙𝒂𝒎𝒑𝒍𝒆,</h3>

<ul>
 <h3>→ 𝑻𝒐 𝒂𝒅𝒅 𝑨 𝒕𝒐 𝑩 𝒘𝒆 𝒄𝒂𝒏 𝒘𝒓𝒊𝒕𝒆 𝒂𝒔 𝑨𝑩 + 𝒐𝒓 𝑩𝑨 + .</h3>
<h3>→ 𝒕𝒐 𝒔𝒖𝒃𝒕𝒓𝒂𝒄𝒕 𝑫 𝒇𝒓𝒐𝒎 𝑪 𝒘𝒆 𝒉𝒂𝒗𝒆 𝒕𝒐 𝒘𝒓𝒊𝒕𝒆 𝒂𝒔 𝑪𝑫 − 𝒏𝒐𝒕 𝒂𝒔
𝑫𝑪 − .</h3>
   
</ul>
    
<h3>𝑰𝒏 𝒐𝒓𝒅𝒆𝒓 𝒕𝒐 𝒕𝒓𝒂𝒏𝒔𝒍𝒂𝒕𝒆 𝒂𝒏 𝒂𝒓𝒊𝒕𝒉𝒎𝒆𝒕𝒊𝒄 𝒆𝒙𝒑𝒓𝒆𝒔𝒔𝒊𝒐𝒏 𝒊𝒏 𝒊𝒏𝒇𝒊𝒙
𝒏𝒐𝒕𝒂𝒕𝒊𝒐𝒏 𝒕𝒐 𝒓𝒆𝒗𝒆𝒓𝒔𝒆 𝒑𝒐𝒍𝒊𝒔𝒉 𝒏𝒐𝒕𝒂𝒕𝒊𝒐𝒏, 𝒘𝒆 𝒅𝒐 𝒔𝒕𝒆𝒑 𝒃𝒚 𝒔𝒕𝒆𝒑
𝒖𝒔𝒊𝒏𝒈 𝒃𝒓𝒂𝒄𝒌𝒆𝒕𝒔([])𝒕𝒐 𝒊𝒏𝒅𝒊𝒄𝒂𝒕𝒆 𝒕𝒉𝒆 𝒑𝒂𝒓𝒕𝒊𝒂𝒍 𝒕𝒓𝒂𝒏𝒔𝒍𝒂𝒕𝒊𝒐𝒏:</h3>
    
<h3>𝑪𝒐𝒏𝒔𝒊𝒅𝒆𝒓 𝒕𝒉𝒆 𝒇𝒐𝒍𝒍𝒐𝒘𝒊𝒏𝒈 𝒆𝒙𝒑𝒓𝒆𝒔𝒔𝒊𝒐𝒏 𝒊𝒏 𝒊𝒏𝒇𝒊𝒙 𝒏𝒐𝒕𝒂𝒕𝒊𝒐𝒏:</h3>
    
 <h3>
	
 ```math
	
 \begin{equation}
   \begin{split}
	
(𝑨 − 𝑩/𝑪) ∗ (𝑨 ∗ 𝑲 − 𝑳)\\	
	
    \end{split}
 \end{equation}
	
```

</h3>
    
    
<h3>𝒕𝒉𝒆 𝒑𝒂𝒓𝒕𝒊𝒂𝒍 𝒕𝒓𝒂𝒏𝒔𝒍𝒂𝒕𝒊𝒐𝒏𝒔 𝒎𝒂𝒚 𝒍𝒐𝒐𝒌 𝒍𝒊𝒌𝒆:</h3>
    
    
  <h3>
	
 ```math
	
 \begin{equation}
   \begin{split}
	
= (𝑨 − [𝑩𝑪/]) ∗ ([𝑨𝑲 ∗] − 𝑳) \\
= [𝑨𝑩𝑪/−] ∗ [𝑨𝑲 ∗ 𝑳−] \\
= 𝑨𝑩𝑪/−𝑨𝑲 ∗ 𝑳 −∗ \\
	
    \end{split}
 \end{equation}
	
```

</h3>
    
    
<h2>𝑬𝒙𝒂𝒎𝒑𝒍𝒆 𝟏 ∶ </h2>
    
<h3>
	
 ```Syntax
		
𝑨 + (𝑩 ∗ 𝑪 − (𝑫/𝑬^𝑭) ∗ 𝑮) ∗ 𝑯 

```

</h3>
    
<h3>𝑷𝒂𝒓𝒕𝒊𝒂𝒍 𝒕𝒓𝒂𝒏𝒔𝒍𝒂𝒕𝒊𝒐𝒏𝒔 𝒐𝒇 𝒕𝒉𝒆 𝒂𝒃𝒐𝒗𝒆:</h3>
  
<ul>
   
<h3>𝟏𝒔𝒕 𝒘𝒆 𝒘𝒊𝒍𝒍 𝒅𝒐 𝒕𝒉𝒆 𝒘𝒐𝒓𝒌 𝒐𝒇 𝑷𝒂𝒓𝒆𝒏𝒕𝒉𝒆𝒔𝒊𝒔.</h3>
<h3>𝑵𝒆𝒙𝒕 𝒘𝒆 𝒘𝒊𝒍𝒍 𝒇𝒐𝒍𝒍𝒐𝒘 𝒕𝒉𝒆 𝒑𝒓𝒆𝒄𝒆𝒅𝒆𝒏𝒄𝒆 𝒕𝒂𝒃𝒍𝒆:</h3>

 ![Screenshot (509)](https://github.com/AvinandanBose/ArithmeticExp_Infix_Prefix_Postfix_Theory/assets/38869235/48e06f23-b88f-4ef2-a539-98d4de1d10d9)
  
<h3>𝑯𝒊𝒈𝒉𝒆𝒔𝒕 𝒑𝒓𝒆𝒄𝒆𝒅𝒆𝒏𝒄𝒆 𝒘𝒊𝒍𝒍 𝒃𝒆 𝒆𝒙𝒆𝒄𝒖𝒕𝒆𝒅 𝒇𝒊𝒓𝒔𝒕 𝒂𝒏𝒅 𝒍𝒐𝒘𝒆𝒔𝒕 𝒂𝒕 𝒍𝒂𝒔𝒕.</h3>


</ul>
    
<h3>
	
 ```Syntax
		
= 𝑨 + (𝑩 ∗ 𝑪 − ([𝑫/𝑬𝑭^]) ∗ 𝑮) ∗ 𝑯
= 𝑨 + (𝑩 ∗ 𝑪 − ([𝑫𝑬𝑭^/]) ∗ 𝑮) ∗ 𝑯
= 𝑨 + (𝑩 ∗ 𝑪 − [𝑫𝑬𝑭^/𝑮 ∗]) ∗ 𝑯
= 𝑨 + ([𝑩𝑪 ∗] − 𝑫𝑬𝑭^/𝑮 ∗) ∗ 𝑯
= 𝑨 + (𝑩𝑪 ∗ 𝑫𝑬𝑭^/𝑮 ∗ −) ∗ 𝑯
= 𝑨 + [𝑩𝑪 ∗ 𝑫𝑬𝑭^/𝑮 ∗ −𝑯 ∗]
= [𝑨𝑩𝑪 ∗ 𝑫𝑬𝑭^/𝑮 ∗ −𝑯 ∗ +]
= 𝑨𝑩𝑪 ∗ 𝑫𝑬𝑭^/𝑮 ∗ −𝑯 ∗ +

```

</h3>

<h2><ins>𝑬𝒙𝒂𝒎𝒑𝒍𝒆  𝟐:</ins></h2>
    
    
<h3>
	
 ```Syntax
		
 𝑨 + (𝑩 ∗ 𝑪 − (𝑫/𝑬 + 𝑭) ∗ 𝑮) ∗ 𝑯
= 𝑨 + (𝑩 ∗ 𝑪 − ([𝑫𝑬/] + 𝑭) ∗ 𝑮) ∗ 𝑯
= 𝑨 + (𝑩 ∗ 𝑪 − ([𝑫𝑬/𝑭+]) ∗ 𝑮) ∗ 𝑯
= 𝑨 + (𝑩 ∗ 𝑪 − [𝑫𝑬/𝑭 + 𝑮 ∗]) ∗ 𝑯
= 𝑨 + ([𝑩𝑪 ∗] − 𝑫𝑬/𝑭 + 𝑮 ∗) ∗ 𝑯
= 𝑨 + (𝑩𝑪 ∗ 𝑫𝑬/𝑭 + 𝑮 ∗ −) ∗ 𝑯
= 𝑨 + [𝑩𝑪 ∗ 𝑫𝑬/𝑭 + 𝑮 ∗ −𝑯 ∗]
= [𝑨𝑩𝑪 ∗ 𝑫𝑬/𝑭 + 𝑮 ∗ −𝑯 ∗ +]
= 𝑨𝑩𝑪 ∗ 𝑫𝑬/𝑭 + 𝑮 ∗ −𝑯 ∗ +

```

</h3>

    
  </ul>
  
